lawyer/nonblocking/examples/queue/simple_queue_spec.v
@@ -1,0 +1,33 @@
+From iris.base_logic Require Export gen_heap.
+From iris.proofmode Require Import tactics coq_tactics.
+From iris.bi.lib Require Import fixpoint.
+From trillium.program_logic Require Export weakestpre adequacy ectx_lifting.
+From fairness Require Import utils.
+From lawyer.examples Require Import obls_tactics.
+From lawyer.obligations Require Import obligations_model obligations_resources obligations_am obligations_em obligations_logic env_helpers.
+From lawyer Require Import sub_action_em program_logic.
+From iris.algebra Require Import auth gmap gset excl excl_auth csum mono_nat.
+From iris.base_logic.lib Require Import invariants.
+From lawyer.nonblocking.examples.queue Require Import simple_queue_utils simple_queue init_queue.
+From lawyer.nonblocking.examples.queue.dequeuer Require Import dequeuer_thread. 
+From lawyer.nonblocking.examples.queue.enqueuer Require Import enqueuer_thread. 
+From heap_lang Require Import heap_lang_defs lang notation.
+From lawyer.nonblocking.tokens Require Import om_wfree_inst_tokens. 
+
+Close Scope Z.
+
+Section QueueSpec.
+  Context (SQ: SimpleQueue).
+  Context (ph pfl: loc).
+
+  Definition queue_ms: gmultiset val := {[+ enqueuer_thread SQ; dequeuer_thread SQ +]}.
+
+  Definition queue_Σ: gFunctors := #[
+
+  ].
+
+  Program Definition SimpleQueue_WaitFreeToken: WaitFreeSpecToken queue_ms := {|
+    wfst_is_init_st := is_init_queue_cfg SQ ph pfl #0;
+    wfst_preG := QueuePreG;
+    wfst_G := QueueG;
+  |}.
